adding some comments and cleaning up some of the functions

Dafny/multisegment.dfy
@@ -10,7 +10,7 @@ module Multisegment{
 
     ghost predicate IsLadder(m : Multisegment){
         exists enumeration : Multisegment :: 
-            multiset(enumeration) == multiset(m) &&
+            multiset(enumeration) == multiset(m) &&         //multiset is a built-in function. initialization looks like: multiset{1, 2, 1, 3}
             |enumeration| == |m| &&
             forall index: int ::
                 0 <= index < |m| - 1 ==>
@@ -18,13 +18,15 @@ module Multisegment{
     }
 
 
+
     ghost function depth(i : int, m : Multisegment): int
         requires 0 <= i < |m|
     {
-        MaxOf({0} + (set j: int | 0 <= j < |m| &&
+        MaxOf({0} + (set j: int | 0 <= j < |m| &&                   //{0} is artifically added because we need to satisfy the precondition of MaxOf which asserts that the set is nonempty
             exists s: seq<Segment> :: |s| == j + 1 && 
             multiset(s) <= multiset(m) && IsLadder(s) && s[0] == m[i]))
     }
+
 
 
     ghost function d(m : Multisegment): int
@@ -34,32 +36,29 @@ module Multisegment{
     }
 
 
-    ghost function bucket(m : Multisegment, k : int): set<int>
+
+    ghost function bucket(m : Multisegment, d : int): set<int>
     {
-        set index: int | 0 <= index < |m| && depth(index, m) == k
+        set index: int | 0 <= index < |m| && depth(index, m) == d
     }
 
 
-    ghost predicate IsAdmissible(m : Multisegment, k : int, e : seq<int>)
+
+    ghost predicate IsAdmissible(m : Multisegment, k : int, enumeration : seq<int>)           //checks if a given sequence of indices constitutes an admissible enumeration of bucket(k)
         requires |m| > 0 && 0 <= k <= d(m)
     {
-        SeqToSet(e) == bucket(m, k)
-        && |e| == |bucket(m, k)|
-        && (forall j : int :: 0 <= j < |e| ==> 0 <= e[j] < |m|)
-        && (forall j : int :: 0 <= j < |e| - 1 ==> Precedes(m[e[j+1]], m[e[j]]))
+        SeqToSet(enumeration) == bucket(m, k)         //SeqToSet is a function from utils -- check if the enumeration indices are those of the bucket's
+        && |enumeration| == |bucket(m, k)|              //making sure enumeration does not have duplicates
+        && (forall j : int :: 0 <= j < |enumeration| ==> 0 <= enumeration[j] < |m|)     //making sure enumeration is a sequence of indices into m (none out-of-range)
+        && (forall j : int :: 0 <= j < |enumeration| - 1 ==> Precedes(m[enumeration[j+1]], m[enumeration[j]]))
     }
 
 
-    ghost function {:axiom} AdmissibleEnumeration(m : Multisegment, k : int): (e : seq<int>)
-        ensures SeqToSet(e) == bucket(m, k)
-        ensures |e| == |bucket(m, k)|
-        ensures forall q : int :: 0 <= q < |e| ==> 0 <= e[q] < |m|
 
-
-
-    lemma {:axiom} AdmissibleEnumerationIsAdmissible(m : Multisegment, k : int)
+    ghost function {:axiom} AdmissibleEnumeration(m : Multisegment, k : int): (e : seq<int>)  //a function with the following postconditions exists
         requires |m| > 0 && 0 <= k <= d(m)
         ensures IsAdmissible(m, k, AdmissibleEnumeration(m, k))
+
 
 
     ghost function IndexOf(e : seq<int>, x : int): int
@@ -71,14 +70,16 @@ module Multisegment{
     }
 
 
+    //returns the position of the index i inside the admissible enumeration of its own depth bucket.
     ghost function {:axiom} Position(m : Multisegment, i : int): (p : int)
-        requires 0 <= i < |m|
+        requires 0 <= i < |m| && 0 <= depth(i, m) <= d(m)
         ensures 0 <= p < |AdmissibleEnumeration(m, depth(i, m))|
         ensures AdmissibleEnumeration(m, depth(i, m))[p] == i
 
 
+
     ghost function IVee(m : Multisegment, i : int): (j : int)
-        requires 0 <= i < |m|
+        requires 0 <= i < |m| && 0 <= depth(i, m) <= d(m)
         ensures 0 <= j < |m|
     {
         var e := AdmissibleEnumeration(m, depth(i, m));
@@ -90,13 +91,14 @@ module Multisegment{
 
 
     lemma {:axiom} IVeeRange(m : Multisegment, i : int) 
-        requires 0 <= i < |m|
+        requires 0 <= i < |m| && 0 <= depth(i, m) <= d(m)
         ensures 0 <= IVee(m, i) < |m|
         ensures m[i].0 <= m[IVee(m, i)].1
 
 
+
     ghost function TransformedSegment(m : Multisegment, i : int): Segment
-        requires 0 <= i < |m|
+        requires 0 <= i < |m| && 0 <= depth(i, m) <= d(m)
     {
         IVeeRange(m, i);
         (m[i].0, m[IVee(m, i)].1)
@@ -154,7 +156,7 @@ module Multisegment{
 
 
     ghost function HighestLadderFrom(m : Multisegment, i : int): Multisegment
-        requires 0 <= i <= |m|
+        requires 0 <= i <= |m| 
         decreases |m| - i
     {
         if i == |m| then []
@@ -163,6 +165,8 @@ module Multisegment{
         else
             HighestLadderFrom(m, i + 1)
     }
+
+
 
     ghost function l(m : Multisegment): Multisegment
         requires |m| > 0
@@ -183,6 +187,8 @@ module Multisegment{
             DerivedMultisegmentFrom(m, i + 1)
     }
 
+
+
     ghost function DerivedMultisegment(m : Multisegment): Multisegment
         requires |m| > 0
     {
@@ -198,6 +204,7 @@ module Multisegment{
         }
 
 
+
     ghost predicate IsFirstLeadingIndex(m : Multisegment, i : int)
     {
         0 <= i < |m|
@@ -206,9 +213,12 @@ module Multisegment{
     }
 
 
+
     ghost function {:axiom} FirstLeadingIndex(m : Multisegment): (i : int)
         requires |m| > 0
         ensures IsFirstLeadingIndex(m, i)
+
+
 
     ghost function NextCandidates(m : Multisegment, current : int): set<int>
         requires 0 <= current < |m|
@@ -219,11 +229,14 @@ module Multisegment{
             && m[i].0 == m[current].0 + 1
     }
 
+
+
     ghost function {:axiom} NextLeadingIndex(m : Multisegment, current : int): (next : int)
         requires 0 <= current < |m|
         requires NextCandidates(m, current) != {}
         ensures next in NextCandidates(m, current)
         ensures forall i : int :: i in NextCandidates(m, current) ==> m[next].1 <= m[i].1
+
 
 
     ghost function LeadingIndicesFrom(m : Multisegment, current : int, fuel : nat): seq<int>
@@ -235,6 +248,7 @@ module Multisegment{
             var next := NextLeadingIndex(m, current);
             [next] + LeadingIndicesFrom(m, next, fuel - 1)
     }
+
 
 
     ghost function LeadingIndices(m : Multisegment): seq<int>
@@ -254,6 +268,7 @@ module Multisegment{
     }
 
 
+
     ghost function DeltaCircle(m : Multisegment): Segment
         requires |m| > 0
     {
@@ -261,6 +276,7 @@ module Multisegment{
         var i1 := FirstLeadingIndex(m);
         (m[i1].0, m[i1].0 + |LeadingIndices(m)| - 1)
     }
+
 
 
     ghost function DeltaStar(m : Multisegment, i : int): Multisegment
@@ -275,6 +291,7 @@ module Multisegment{
     }
 
 
+
     ghost function MCrossFrom(m : Multisegment, i : int): Multisegment
         requires |m| > 0
         requires 0 <= i <= |m|
@@ -285,11 +302,13 @@ module Multisegment{
     }
 
 
+
     ghost function MCross(m : Multisegment): Multisegment
         requires |m| > 0
     {
         MCrossFrom(m, 0)
     }
+
 
 
     ghost function MW(m : Multisegment): (Multisegment, Segment)
@@ -299,6 +318,7 @@ module Multisegment{
         }
 
 
+
     ghost function min(m : Multisegment): int
         requires |m| > 0
     {
@@ -306,15 +326,14 @@ module Multisegment{
     }
 
 
-
-lemma {:axiom} Corollary(m : Multisegment)
-    requires |m| > 0
-    requires |l(m)| > 0
-    requires min(m) < min(l(m))
-    ensures
-        |DerivedMultisegment(m)| > 0
-        && |MCross(m)| > 0
-        && l(m) == l(MCross(m))
-        && DeltaCircle(m) == DeltaCircle(DerivedMultisegment(m))
-        && DerivedMultisegment(MCross(m)) == MCross(DerivedMultisegment(m))
+    lemma {:axiom} Corollary(m : Multisegment)
+        requires |m| > 0
+        requires |l(m)| > 0
+        requires min(m) < min(l(m))
+        ensures
+            |DerivedMultisegment(m)| > 0
+            && |MCross(m)| > 0
+            && l(m) == l(MCross(m))
+            && DeltaCircle(m) == DeltaCircle(DerivedMultisegment(m))
+            && DerivedMultisegment(MCross(m)) == MCross(DerivedMultisegment(m))
 }
